1. Show not only one phase of the two-phase proof but actually a combination of two phases. 2. Show a comparison of our wand method and traditional approach.

wand_demo/bst_lemmas.v
@@ -1,4 +1,5 @@
 Require Import VST.floyd.proofauto.
+Require Import VFA.Maps.
 Require Import VFA.SearchTree.
 Require Import WandDemo.SearchTree_ext.
 Require Import WandDemo.wand_frame.
@@ -33,7 +34,7 @@ Lemma tree_rep_spec: forall (t: tree val) (p: val),
 Proof.
   intros.
   destruct t; auto.
-Qed.  
+Qed.
 
 Lemma treebox_rep_spec: forall (t: tree val) (b: val),
   treebox_rep t b =
@@ -188,6 +189,80 @@ Proof.
   entailer!.
 Qed.
 
+Module PartialTreeboxRep_WandQFrame_Func_Hole.
+
+Definition partial_treebox_rep (pt: tree val -> tree val) (p_root p_in: val): mpred :=
+  ALL t: tree val, treebox_rep t p_in -* treebox_rep (pt t) p_root.
+
+Lemma partial_treebox_rep_singleton_left: forall (t2: tree val) k (v p b: val),
+  Int.min_signed <= Z.of_nat k <= Int.max_signed ->
+  is_pointer_or_null v ->
+  data_at Tsh (tptr t_struct_tree) p b *
+  field_at Tsh t_struct_tree [StructField _key] (Vint (Int.repr (Z.of_nat k))) p *
+  field_at Tsh t_struct_tree [StructField _value] v p *
+  treebox_rep t2 (field_address t_struct_tree [StructField _right] p)
+  |-- partial_treebox_rep (fun t1 => T t1 k v t2) b (field_address t_struct_tree [StructField _left] p).
+Proof.
+  intros.
+  unfold partial_treebox_rep.
+  apply allp_right; intros t1.
+  rewrite <- wand_sepcon_adjoint.
+  rewrite (treebox_rep_spec (T t1 k v t2)).
+  Exists p.
+  entailer!.
+Qed.
+
+Lemma partial_treebox_rep_singleton_right: forall (t1: tree val) k (v p b: val),
+  Int.min_signed <= Z.of_nat k <= Int.max_signed ->
+  is_pointer_or_null v ->
+  data_at Tsh (tptr t_struct_tree) p b *
+  field_at Tsh t_struct_tree [StructField _key] (Vint (Int.repr (Z.of_nat k))) p *
+  field_at Tsh t_struct_tree [StructField _value] v p *
+  treebox_rep t1 (field_address t_struct_tree [StructField _left] p)
+  |-- partial_treebox_rep (fun t2 => T t1 k v t2) b (field_address t_struct_tree [StructField _right] p).
+Proof.
+  intros.
+  unfold partial_treebox_rep.
+  apply allp_right; intros t2.
+  rewrite <- wand_sepcon_adjoint.
+  rewrite (treebox_rep_spec (T t1 k v t2)).
+  Exists p.
+  entailer!.
+Qed.
+
+Lemma partial_treebox_rep_partial_treebox_rep: forall pt12 pt23 p1 p2 p3,
+  partial_treebox_rep pt12 p2 p1 * partial_treebox_rep pt23 p3 p2 |-- partial_treebox_rep (Basics.compose pt23 pt12) p3 p1.
+Proof.
+  intros.
+  unfold partial_treebox_rep.
+  sep_apply (wandQ_frame_refine _ _ (fun t => treebox_rep t p2 -* treebox_rep (pt23 t) p3) pt12).
+  rewrite sepcon_comm.
+  apply wandQ_frame_ver.
+Qed.
+
+Lemma emp_partial_treebox_rep_H: forall p,
+  emp |-- partial_treebox_rep (fun t => t) p p.
+Proof.
+  intros.
+  apply allp_right; intros.
+  apply wand_sepcon_adjoint.
+  normalize.
+Qed.
+
+Lemma treebox_rep_partial_treebox_rep: forall t pt p q,
+  treebox_rep t p * partial_treebox_rep pt q p |-- treebox_rep (pt t) q.
+Proof.
+  intros.
+  unfold partial_treebox_rep.
+  change (treebox_rep (pt t) q)
+    with ((fun t => treebox_rep (pt t) q) t).
+  change (treebox_rep t p)
+    with ((fun t => treebox_rep t p) t).
+  apply wandQ_frame_elim.
+Qed.
+
+End PartialTreeboxRep_WandQFrame_Func_Hole.
+
 Module PartialTreeboxRep_WandFrame.
 
 Lemma partial_treebox_rep_singleton_left: forall (t1' t2: tree val) k (v p b: val),
@@ -250,7 +325,7 @@ Qed.
 
 End PartialTreeboxRep_WandFrame.
 
-Module PartialTreeboxRep_WandQFrame.
+Module PartialTreeboxRep_WandQFrame_Ind_Hole.
 
 Definition partial_treebox_rep (pt: partial_tree val) (p_root p_in: val): mpred :=
   ALL t: tree val, treebox_rep t p_in -* treebox_rep (partial_tree_tree pt t) p_root.
@@ -323,12 +398,30 @@ Proof.
   apply wandQ_frame_elim.
 Qed.
 
-End PartialTreeboxRep_WandQFrame.
+End PartialTreeboxRep_WandQFrame_Ind_Hole.
 
-Module PartialTreeboxRep_WandQFrame'.
+Module PartialTreeboxRep_Ind_Pred_Ind_Hole.
 
-Definition partial_treebox_rep (pt: tree val -> tree val) (p_root p_in: val): mpred :=
-  ALL t: tree val, treebox_rep t p_in -* treebox_rep (pt t) p_root.
+Fixpoint partial_treebox_rep (pt: partial_tree val) (p_root p_in: val): mpred :=
+  match pt with
+  | H => !! (p_root = p_in) && emp
+  | L pt1 x v t2 =>
+      EX p : val,
+        !! (Int.min_signed <= Z.of_nat x <= Int.max_signed /\ tc_val (tptr Tvoid) v) &&
+        data_at Tsh (tptr t_struct_tree) p p_root *
+        field_at Tsh t_struct_tree [StructField _key] (Vint (Int.repr (Z.of_nat x))) p *
+        field_at Tsh t_struct_tree [StructField _value] v p *
+        partial_treebox_rep pt1 (field_address t_struct_tree [StructField _left] p) p_in *
+        treebox_rep t2 (field_address t_struct_tree [StructField _right] p)
+  | R t1 x v pt2 =>
+      EX p : val,
+        !! (Int.min_signed <= Z.of_nat x <= Int.max_signed /\ tc_val (tptr Tvoid) v) &&
+        data_at Tsh (tptr t_struct_tree) p p_root *
+        field_at Tsh t_struct_tree [StructField _key] (Vint (Int.repr (Z.of_nat x))) p *
+        field_at Tsh t_struct_tree [StructField _value] v p *
+        treebox_rep t1 (field_address t_struct_tree [StructField _left] p) *
+        partial_treebox_rep pt2 (field_address t_struct_tree [StructField _right] p) p_in
+  end.
 
 Lemma partial_treebox_rep_singleton_left: forall (t2: tree val) k (v p b: val),
   Int.min_signed <= Z.of_nat k <= Int.max_signed ->
@@ -337,13 +430,10 @@ Lemma partial_treebox_rep_singleton_left: forall (t2: tree val) k (v p b: val),
   field_at Tsh t_struct_tree [StructField _key] (Vint (Int.repr (Z.of_nat k))) p *
   field_at Tsh t_struct_tree [StructField _value] v p *
   treebox_rep t2 (field_address t_struct_tree [StructField _right] p)
-  |-- partial_treebox_rep (fun t1 => T t1 k v t2) b (field_address t_struct_tree [StructField _left] p).
+  |-- partial_treebox_rep (L H k v t2) b (field_address t_struct_tree [StructField _left] p).
 Proof.
   intros.
   unfold partial_treebox_rep.
-  apply allp_right; intros t1.
-  rewrite <- wand_sepcon_adjoint.
-  rewrite (treebox_rep_spec (T t1 k v t2)).
   Exists p.
   entailer!.
 Qed.
@@ -355,46 +445,63 @@ Lemma partial_treebox_rep_singleton_right: forall (t1: tree val) k (v p b: val),
   field_at Tsh t_struct_tree [StructField _key] (Vint (Int.repr (Z.of_nat k))) p *
   field_at Tsh t_struct_tree [StructField _value] v p *
   treebox_rep t1 (field_address t_struct_tree [StructField _left] p)
-  |-- partial_treebox_rep (fun t2 => T t1 k v t2) b (field_address t_struct_tree [StructField _right] p).
+  |-- partial_treebox_rep (R t1 k v H) b (field_address t_struct_tree [StructField _right] p).
 Proof.
   intros.
   unfold partial_treebox_rep.
-  apply allp_right; intros t2.
-  rewrite <- wand_sepcon_adjoint.
-  rewrite (treebox_rep_spec (T t1 k v t2)).
   Exists p.
   entailer!.
 Qed.
 
 Lemma partial_treebox_rep_partial_treebox_rep: forall pt12 pt23 p1 p2 p3,
-  partial_treebox_rep pt12 p2 p1 * partial_treebox_rep pt23 p3 p2 |-- partial_treebox_rep (Basics.compose pt23 pt12) p3 p1.
+  partial_treebox_rep pt12 p2 p1 * partial_treebox_rep pt23 p3 p2 |-- partial_treebox_rep (partial_tree_partial_tree pt23 pt12) p3 p1.
 Proof.
   intros.
-  unfold partial_treebox_rep.
-  sep_apply (wandQ_frame_refine _ _ (fun t => treebox_rep t p2 -* treebox_rep (pt23 t) p3) pt12).
-  rewrite sepcon_comm.
-  apply wandQ_frame_ver.
+  revert p3; induction pt23; intros.
+  + simpl.
+    entailer!.
+  + simpl.
+    Intros p.
+    Exists p.
+    entailer!.
+    apply IHpt23.
+  + simpl.
+    Intros p.
+    Exists p.
+    entailer!.
+    apply IHpt23.
 Qed.
 
 Lemma emp_partial_treebox_rep_H: forall p,
-  emp |-- partial_treebox_rep (fun t => t) p p.
-Proof.
-  intros.
-  apply allp_right; intros.
-  apply wand_sepcon_adjoint.
-  normalize.
-Qed.
-
-Lemma treebox_rep_partial_treebox_rep: forall t pt p q,
-  treebox_rep t p * partial_treebox_rep pt q p |-- treebox_rep (pt t) q.
+  emp |-- partial_treebox_rep H p p.
 Proof.
   intros.
   unfold partial_treebox_rep.
-  change (treebox_rep (pt t) q)
-    with ((fun t => treebox_rep (pt t) q) t).
-  change (treebox_rep t p)
-    with ((fun t => treebox_rep t p) t).
-  apply wandQ_frame_elim.
+  entailer!.
 Qed.
 
-End PartialTreeboxRep_WandQFrame'.
+Lemma treebox_rep_partial_treebox_rep: forall t pt p q,
+  treebox_rep t p * partial_treebox_rep pt q p |-- treebox_rep (partial_tree_tree pt t) q.
+Proof.
+  intros.
+  revert q; induction pt; intros.
+  + simpl.
+    entailer!.
+  + simpl.
+    Intros p'.
+    rewrite (treebox_rep_spec (T (partial_tree_tree pt t) k v t0)).
+    Exists p'.
+    entailer!.
+    apply IHpt.
+  + simpl.
+    Intros p'.
+    rewrite (treebox_rep_spec (T t0 k v (partial_tree_tree pt t))).
+    Exists p'.
+    entailer!.
+    apply IHpt.
+Qed.
+
+End PartialTreeboxRep_Ind_Pred_Ind_Hole.
+
+Definition Map_rep (m: total_map val) (p: val): mpred :=
+  EX t: tree val, !! (Abs val nullval t m /\ SearchTree val t) && treebox_rep t p.
